theories/Interpreter.v
@@ -27,27 +27,31 @@ Inductive Interpret context term : Context.context -> Term.term -> Prop :=
 
 
 
+Definition penalty_for_incompatible_match context t :=
+  match t with
+  | Term.App function argument =>
+      match function with
+      | Term.Cas pattern body_if_match other_cases =>
+          let clean := andb (Match.compatible context pattern) $ Unshadow.unshadowed $ Term.App function argument in
+          if clean then 0 else 1
+      | _ => 0
+      end
+  | _ => 0
+  end.
+
 Instance wf : Classes.WellFounded $ Telescopes.tele_measure
   (Telescopes.ext Context.context (fun _ => Telescopes.tip Term.term)) nat
-  (fun context term => Term.nodes term + List.fold_right (fun kv =>
-    Nat.add $ Term.nodes $ snd kv) 0 (MapCore.bindings context)) lt.
+    (fun context term => (* penalty_for_incompatible_match context term + *) Term.nodes term +
+    List.fold_right (fun kv => Nat.add $ Term.nodes $ snd kv) 0 (MapCore.bindings context)) lt.
 Proof. apply Telescopes.wf_tele_measure. exact Subterm.lt_wf. Qed.
 
-Lemma pull_out_of_acc add acc (li : list (MapCore.key * Term.term))
-  : List.fold_right (fun kv => Nat.add $ Term.nodes $ snd kv) (add + acc) li =
-    add + List.fold_right (fun kv => Nat.add $ Term.nodes $ snd kv) acc li.
-Proof.
-  generalize dependent acc. generalize dependent add.
-  induction li as [| [k v] tail IH]; intros; cbn in *. { reflexivity. }
-  rewrite PeanoNat.Nat.add_assoc. rewrite (PeanoNat.Nat.add_comm add $ Term.nodes v).
-  rewrite <- PeanoNat.Nat.add_assoc. f_equal. apply IH.
-Qed.
 
 
 (*
 Equations interpret (context : Context.context) (term : Term.term)
-  : Context.context * Term.term by wf (Nat.add (Term.nodes term) $
-    List.fold_right (fun kv => Nat.add $ Term.nodes $ snd kv) 0 $ MapCore.bindings context) lt :=
+  : Context.context * Term.term by wf (
+    (* penalty_for_incompatible_match context term + *) Term.nodes term +
+    List.fold_right (fun kv => Nat.add $ Term.nodes $ snd kv) 0 (MapCore.bindings context)) lt :=
   interpret context term with SmallStepFunction.dec context term => {
     | @SmallStepFunction.CouldntStep _ => (context, term)
     | @SmallStepFunction.Stepped _ _ context' term' _ => interpret context' term'
@@ -57,72 +61,38 @@ Next Obligation.
   - cbn. destruct no_contraction as [_ R]. assert (R' := Map.remove_if_present_remove name context).
     eapply Map.remove_if_present_det in R'. 2: { exact R. } 2: { reflexivity. } 2: { apply Map.eq_refl. }
     apply Map.bindings_eq in R' as ->. destruct (Map.bindings_remove_split lookup) as [bl [br [-> ->]]].
-    repeat rewrite List.fold_right_app. cbn. rewrite pull_out_of_acc. apply PeanoNat.Nat.lt_succ_diag_r.
+    repeat rewrite List.fold_right_app. cbn. rewrite Match.pull_out_of_acc. (* rewrite <- PeanoNat.Nat.add_assoc.
+    rewrite <- PeanoNat.Nat.add_1_l. apply PeanoNat.Nat.add_lt_mono_r. *) apply PeanoNat.Nat.lt_succ_diag_r.
   - apply PeanoNat.Nat.add_lt_mono_l. eassert (agree : _); [| assert (A :=
       @Map.add_overriding _ self stepped updated_context_without_self agree)]. {
       intros v' F'. contradiction not_overwriting_self. eexists. exact F'. }
     eapply Map.add_det in A. 2: { exact update. } 2: { reflexivity. } 2: { reflexivity. } 2: { apply Map.eq_refl. }
     apply Map.bindings_eq in A as ->. destruct (Map.bindings_add_split not_overwriting_self stepped) as [bl [br [Ea Eu]]].
-    rewrite Ea. rewrite List.fold_right_app. cbn. rewrite pull_out_of_acc.
+    rewrite Ea. rewrite List.fold_right_app. cbn. rewrite Match.pull_out_of_acc.
     rewrite <- List.fold_right_app. rewrite <- Eu. clear Ea Eu.
     destruct remove_self_from_context as [_ R]. assert (R' := Map.remove_if_present_remove self context).
     eapply Map.remove_if_present_det in R'. 2: { exact R. } 2: { reflexivity. } 2: { apply Map.eq_refl. }
     apply Map.bindings_eq in R'. rewrite R' in IHstepped. destruct (Map.bindings_remove_split lookup) as [bl' [br' [-> Er]]].
-    rewrite Er in IHstepped. rewrite List.fold_right_app in *; simpl List.fold_right in *. rewrite pull_out_of_acc. exact IHstepped.
+    rewrite Er in IHstepped. rewrite List.fold_right_app in *; simpl List.fold_right in *. rewrite Match.pull_out_of_acc. exact IHstepped.
   - cbn. apply -> PeanoNat.Nat.succ_lt_mono. repeat rewrite (PeanoNat.Nat.add_comm _ $ Term.nodes argument).
     repeat rewrite <- PeanoNat.Nat.add_assoc. apply PeanoNat.Nat.add_lt_mono_l. exact IHstepped.
-  - clear compatible_names unshadowed. cbn. repeat rewrite <- (PeanoNat.Nat.add_assoc $ Term.nodes body_if_match).
-    do 2 rewrite plus_n_Sm. apply PeanoNat.Nat.add_lt_mono_l. clear body_if_match. invert matched.
-    + rename S into A. eassert (agree : _); [| assert (A' := @Map.add_overriding _ name scrutinee context agree)]. {
-        intros v' F'. contradiction N. eexists. exact F'. }
-      eapply Map.add_det in A'. 2: { exact A. } 2: { reflexivity. } 2: { reflexivity. } 2: { apply Map.eq_refl. }
-      apply Map.bindings_eq in A' as ->. destruct (Map.bindings_add_split N scrutinee) as [bl [br [-> ->]]].
-      repeat rewrite List.fold_right_app; cbn. rewrite pull_out_of_acc.
-      rewrite (PeanoNat.Nat.add_comm _ $ Term.nodes scrutinee). rewrite <- PeanoNat.Nat.add_assoc. do 2 rewrite plus_n_Sm.
-      apply PeanoNat.Nat.add_lt_mono_l. repeat rewrite <- PeanoNat.Nat.add_succ_l.
-      apply PeanoNat.Nat.lt_add_pos_l. apply PeanoNat.Nat.lt_0_succ.
-    + invert move_or_reference_matched; rename S into M.
-      * generalize dependent other_cases. induction M; intros; cbn in *. {
-          rewrite (PeanoNat.Nat.add_comm _ 1). cbn. apply Map.bindings_eq in E as ->.
-          repeat rewrite <- PeanoNat.Nat.add_succ_l. apply PeanoNat.Nat.lt_add_pos_l. apply PeanoNat.Nat.lt_0_succ. }
-        eassert (agree : _); [| assert (A' := @Map.add_overriding _ argument_name argument context_with_function_matches agree)]. {
-          intros y F. contradiction N. eexists. exact F. }
-        eapply Map.add_det in A'; try reflexivity. 2: { exact A. } 2: { apply Map.eq_refl. }
-        apply Map.bindings_eq in A' as ->. destruct (Map.bindings_add_split N argument) as [bl [br [E1 E2]]]. rewrite E1.
-        rewrite List.fold_right_app. cbn. rewrite pull_out_of_acc. rewrite <- List.fold_right_app. rewrite <- E2.
-        rewrite (PeanoNat.Nat.add_comm _ $ Term.nodes argument). rewrite PeanoNat.Nat.add_succ_r. rewrite PeanoNat.Nat.add_assoc.
-        rewrite (PeanoNat.Nat.add_comm _ $ Term.nodes argument). rewrite PeanoNat.Nat.add_succ_l.
-        repeat rewrite <- PeanoNat.Nat.add_assoc. repeat rewrite <- (PeanoNat.Nat.add_succ_r $ Term.nodes argument).
-        apply PeanoNat.Nat.add_lt_mono_l. rewrite PeanoNat.Nat.add_assoc. eapply PeanoNat.Nat.lt_trans. { apply IHM. }
-        repeat apply -> PeanoNat.Nat.succ_lt_mono. apply PeanoNat.Nat.lt_succ_diag_r.
-      * invert follow_references. 2: { edestruct N as []. reflexivity. } clear term F transitive without_self R.
-        destruct OW as [[looked_up lookup] OW]. assert (OW' := Map.overwrite_if_present_overwrite name old_context_with_matches cleaved).
-        eapply Map.overwrite_if_present_det in OW'; try reflexivity. 2: { exact OW. } 2: { apply Map.eq_refl. }
-        apply Map.bindings_eq in OW' as ->. clear context_with_matches OW. cbn. rewrite (PeanoNat.Nat.add_comm _ 1). cbn.
-        generalize dependent looked_up. generalize dependent name. generalize dependent other_cases.
-        induction M; intros; cbn in *. { apply Map.bindings_eq in E as ->.
-          destruct (Map.bindings_overwrite_split lookup $ Term.Ctr ctor) as [bl [br [E1 ->]]]; cbn in E1; rewrite E1; clear E1.
-          repeat rewrite List.fold_right_app. cbn. rewrite <- PeanoNat.Nat.add_1_l. repeat rewrite pull_out_of_acc. cbn.
-          apply -> PeanoNat.Nat.succ_lt_mono. rewrite PeanoNat.Nat.add_assoc. repeat rewrite <- PeanoNat.Nat.add_succ_l.
-          apply PeanoNat.Nat.lt_add_pos_l. apply PeanoNat.Nat.lt_0_succ. }
-        apply A in lookup as [[-> ->] | lookup]. 2: {
-          rewrite <- (IHM _ _ _ lookup); clear IHM. assert (E : Map.Eq
-            (Map.overriding_add name (Term.App function_cleaved $ Term.Var argument_name Ownership.Owned) context_with_matches)
-            (Map.overriding_add name (Term.App function_cleaved $ Term.Var argument_name Ownership.Owned) $
-              Map.overriding_add argument_name argument context_with_function_matches)). {
-            intros k v. repeat rewrite Map.find_overriding_add. split; (intros [[-> ->] | [N' F]]; [left; split; reflexivity | right]);
-            (split; [exact N' |]). 2: { apply A. destruct F as [E | [Nk F]]; [left | right]; [exact E | exact F]. }
-            apply A in F as [[-> ->] | F]; [left; split; reflexivity | right].
-            split. 2: { exact F. } intros ->. apply N. eexists. exact F. } apply Map.bindings_eq in E as ->.
-          destruct (Map.bindings_overwrite_split lookup function_cleaved) as [bl [br [E1 E2]]]; cbn in E1; rewrite E1; clear E1.
-          rewrite List.fold_right_app. cbn. rewrite pull_out_of_acc. rewrite <- List.fold_right_app.
-          assert (lookup' : Map.Find (Map.overriding_add argument_name argument context_with_function_matches) name looked_up). {
-            apply Map.add_overriding. { intros v' F'. contradiction N. eexists. exact F'. } right. exact lookup. }
-          destruct (Map.bindings_overwrite_split lookup' $ Term.App function_cleaved $ Term.Var argument_name Ownership.Owned)
-            as [bl' [br' [E1' E2']]]; cbn in E1'; rewrite E1'; clear E1' lookup'. rewrite List.fold_right_app. cbn.
-          rewrite (PeanoNat.Nat.add_comm _ 1). rewrite <- PeanoNat.Nat.add_1_l. rewrite PeanoNat.Nat.add_assoc.
-          rewrite pull_out_of_acc. cbn. repeat rewrite <- PeanoNat.Nat.add_succ_r. apply PeanoNat.Nat.add_lt_mono_l.
-          rewrite <- List.fold_right_app. Abort.
+  - clear compatible_names unshadowed. cbn. rewrite (PeanoNat.Nat.add_comm $ Pattern.nodes _).
+    repeat rewrite <- (PeanoNat.Nat.add_assoc $ Term.nodes body_if_match). repeat rewrite (plus_n_Sm $ Term.nodes _).
+    apply PeanoNat.Nat.add_lt_mono_l. clear body_if_match. eapply PeanoNat.Nat.lt_trans. { eapply Match.decreasing. exact matched. }
+    eapply PeanoNat.Nat.lt_trans; apply PeanoNat.Nat.lt_succ_diag_r.
+  - cbn. repeat apply -> PeanoNat.Nat.succ_lt_mono. repeat rewrite <- PeanoNat.Nat.add_assoc.
+    repeat apply PeanoNat.Nat.add_lt_mono_l. exact IHstepped.
+  - cbn. apply -> PeanoNat.Nat.succ_lt_mono. rewrite <- (PeanoNat.Nat.add_assoc $ Pattern.nodes _).
+    rewrite (PeanoNat.Nat.add_comm _ $ Term.nodes other_cases). rewrite PeanoNat.Nat.add_assoc.
+    rewrite (PeanoNat.Nat.add_comm _ $ Term.nodes other_cases). repeat rewrite <- PeanoNat.Nat.add_assoc.
+    rewrite <- PeanoNat.Nat.add_succ_r. apply PeanoNat.Nat.add_lt_mono_l.
+    rewrite (PeanoNat.Nat.add_assoc _ $ Term.nodes scrutinee). rewrite (PeanoNat.Nat.add_comm _ $ Term.nodes scrutinee).
+    repeat rewrite PeanoNat.Nat.add_assoc. rewrite (PeanoNat.Nat.add_comm _ $ Term.nodes scrutinee).
+    repeat rewrite <- PeanoNat.Nat.add_assoc. rewrite <- PeanoNat.Nat.add_succ_r. apply PeanoNat.Nat.add_lt_mono_l.
+    repeat rewrite PeanoNat.Nat.add_assoc. rewrite <- PeanoNat.Nat.add_succ_l.
+    apply Map.bindings_eq in context_unchanged as ->. apply PeanoNat.Nat.lt_add_pos_l. apply PeanoNat.Nat.lt_0_succ.
+  - apply Map.bindings_eq in context_unchanged as <-; clear unchanged_context.
+    apply Unshadow.nodes_eq_reserve in rename as ->; clear context_domain D renamed. cbn. Abort.
 Fail Next Obligation.
 
 
@@ -132,4 +102,5 @@ Theorem terminating context term
 Proof.
   destruct (interpret context term) as [context' term'] eqn:I.
   exists context'. exists term'. apply interpret_iff. exact I.
-Qed. *)
+Qed.
+*)
