theories/Shape.v
@@ -8,6 +8,7 @@ From LinearCore Require
   Term
   .
 From LinearCore Require Import
+  DollarSign
   Invert
   .
 
@@ -68,80 +69,54 @@ Qed.
 
 
 
-Inductive ShapeOrRef context : Term.term -> shape -> Prop :=
-  | RCtr ctor
-      : ShapeOrRef context (Term.Ctr ctor) Resource
-  | RRef {name term} (F : Map.Find context name term)
-      {without_self} (R : Map.Remove name context without_self)
-      {shape} (S : ShapeOrRef without_self term shape)
-      : ShapeOrRef context (Term.Var name Ownership.Referenced) shape
-  | RApp {curried} (curried_resource : ShapeOf curried Resource) argument
-      : ShapeOrRef context (Term.App curried argument) Resource
-  | RCas pattern body_if_match other_cases
-      : ShapeOrRef context (Term.Cas pattern body_if_match other_cases) Function
+Variant ShapeOrRef context : Term.term -> shape -> Prop :=
+  | RRef {symlink real_name looked_up}
+      (follow_references : Context.FollowReferences context symlink real_name looked_up)
+      {shape} (shaped : ShapeOf looked_up shape)
+      : ShapeOrRef context (Term.Var symlink Ownership.Referenced) shape
+  | RDel {term shape} (shaped : ShapeOf term shape)
+      : ShapeOrRef context term shape
   .
 
 Lemma det_ref {c1 t s1} (S1 : ShapeOrRef c1 t s1) {c2}
   (Ec : Map.Eq c1 c2) {s2} (S2 : ShapeOrRef c2 t s2)
   : s1 = s2.
 Proof.
-  generalize dependent s2. generalize dependent c2. induction S1; intros; try solve [invert S2; reflexivity].
-  invert S2. eapply IHS1. 2: { apply Ec in F0. destruct (Map.find_det F F0). exact S. }
-  intros k v. destruct R as [D R]. cbn in R. rewrite R.
-  destruct R0 as [D0 R0]. cbn in R0. rewrite R0. cbn in Ec. rewrite Ec. reflexivity.
+  invert S1. 2: { invert S2. { invert shaped. } eapply det; eassumption. }
+  invert S2. 2: { invert shaped0. }
+  destruct (Context.follow_references_det follow_references Ec eq_refl follow_references0) as [<- <-]. eapply det; eassumption.
 Qed.
 
 Lemma eq_ref {c1 t s1} (S1 : ShapeOrRef c1 t s1) {c2}
   (Ec : Map.Eq c1 c2) {s2} (Es : s1 = s2)
   : ShapeOrRef c2 t s2.
-Proof.
-  generalize dependent s2. generalize dependent c2. induction S1; intros; subst; try solve [constructor].
-  - econstructor. { apply Ec. exact F. } 2: { exact S1. }
-    split. { eexists. apply Ec. exact F. } destruct R as [D R]. cbn in R.
-    intros k v. rewrite R. cbn in Ec. rewrite Ec. reflexivity.
-  - constructor. exact curried_resource.
-Qed.
+Proof. invert S1; econstructor; try eassumption. eapply Context.follow_references_eq; try eassumption; reflexivity. Qed.
+
+Lemma or_ref {t s} (S : ShapeOf t s) context
+  : ShapeOrRef context t s.
+Proof. generalize dependent context. induction S; intros; repeat constructor; exact S. Qed.
 
 
 
-Equations shape_or_ref (context : Context.context) (t : Term.term)
-  : option shape by wf (Map.cardinality context) lt :=
-  shape_or_ref _ (Term.Ctr _) := Some Resource;
-  shape_or_ref context (Term.Var name Ownership.Referenced) with Map.found_dec context name => {
-  | Map.NotFound => None
-  | @Map.Found term _ => shape_or_ref (Map.remove name context) term };
-  shape_or_ref _ (Term.App curried argument) :=
-    match shape_of curried with Some Resource => Some Resource | _ => None end;
-  shape_or_ref _ (Term.Cas _ _ _) := Some Function;
-  shape_or_ref _ _ := None.
-Next Obligation.
-  clear shape_or_ref. rewrite Map.cardinality_remove. apply Map.find_iff in Y as E. rewrite E. clear E.
-  unfold Map.cardinality. rewrite MapCore.cardinal_spec. apply MapCore.bindings_spec1 in Y.
-  remember (MapCore.bindings context) as b eqn:Eb; clear context Eb. destruct b. { invert Y. }
-  cbn. apply PeanoNat.Nat.lt_succ_diag_r. Qed.
-Fail Next Obligation.
+Definition shape_or_ref (context : Context.context) (t : Term.term) :=
+  match t with
+  | Term.Var symlink Ownership.Referenced =>
+      match Context.follow_references context symlink with
+      | None => None
+      | Some (real_name, looked_up) => shape_of looked_up
+      end
+  | _ => shape_of t
+  end.
 
 Lemma shape_or_ref_spec context t
   : Reflect.Option (ShapeOrRef context t) (shape_or_ref context t).
 Proof.
-  funelim (shape_or_ref context t).
-  - constructor. constructor.
-  - constructor. intros s S. invert S.
-  - destruct (shape_of curried) eqn:E. 2: {
-      constructor. intros s S. invert S. apply shape_iff in curried_resource.
-      rewrite E in curried_resource. discriminate curried_resource. }
-    destruct s; constructor. { constructor. apply shape_iff. exact E. }
-    intros s S. invert S. apply shape_iff in curried_resource. rewrite E in curried_resource. invert curried_resource.
-  - constructor. intros s S. invert S.
-  - constructor. constructor.
-  - destruct H; constructor. { econstructor. { exact Y. } { apply Map.remove_remove. eexists. exact Y. } exact Y0. }
-    intros s S. invert S. eapply N. destruct (Map.find_det Y F). eapply eq_ref. { exact S0. } 2: { reflexivity. }
-    eapply Map.remove_det. { exact R. } { reflexivity. } { apply Map.eq_refl. } apply Map.remove_remove. eexists. exact Y.
-  - constructor. intros s S. invert S. apply N in F as [].
+  unfold shape_or_ref. destruct (shape_spec t).
+  - destruct t; try destruct ownership; try solve [constructor; apply or_ref; exact Y]. invert Y.
+  - destruct t; try destruct ownership; try solve [constructor; intros s C; invert C; apply N in shaped as []].
+    destruct (Context.follow_references_spec context name) as [[k v] |]; cbn in *.
+    + destruct (shape_spec v); constructor. { econstructor. { exact Y. } exact Y0. }
+      intros s C. invert C. 2: { invert shaped. }
+      destruct (Context.follow_references_det Y (Map.eq_refl _) eq_refl follow_references) as [<- <-]. apply N0 in shaped as [].
+    + constructor. intros s C. invert C. 2: { invert shaped. } apply (N0 (_, _)) in follow_references as [].
 Qed.
-
-
-
-Lemma or_ref {t s} (S : ShapeOf t s) context
-  : ShapeOrRef context t s.
-Proof. generalize dependent context. induction S; intros. { constructor. } { constructor. exact S. } constructor. Qed.
